theories/Relational/GenericRulesSimple.v
@@ -3,133 +3,134 @@ From Coq Require FunctionalExtensionality.
 From Mon Require Export Base.
 From Mon.SRelation Require Import SRelation_Definitions SMorphisms.
 From Mon.sprop Require Import SPropBase SPropMonadicStructures.
-From Relational Require Import Category RelativeMonads RelativeMonadExamples.
+(* From Relational Require Import Category RelativeMonads RelativeMonadExamples. *)
+From Relational Require Import  OrderEnrichedCategory OrderEnrichedRelativeMonadExamples.
 
 Set Primitive Projections.
 Set Universe Polymorphism.
 
 (* We introduce relational program logic rules starting from abstract algebraic structure *)
 
-Section RelationalProgramLogicFromBimodule.
-  Context (M1 M2 : Monad) (M12 := compPair M1 M2).
-  Context (W : functor TypeCatSq OrdCat) (rmW : rightModuleStructure M12 W).
-  Context (η : natTrans Jprod W) (σ := point_to_homomorphism Jprod rmW η).
+(* Section RelationalProgramLogicFromBimodule. *)
+(*   Context (M1 M2 : Monad) (M12 := compPair M1 M2). *)
+(*   Context (W : ord_functor TypeCatSq OrdCat) (rmW : rightModuleStructure M12 W). *)
+(*   Context (η : natTrans Jprod W) (σ := point_to_homomorphism Jprod rmW η). *)
 
-  Definition mod_semantic_judgement {A1 A2} c1 c2 w := 
-    Spr1 (σ ⟨A1,A2⟩) ⟨c1,c2⟩ ≤ w.
+(*   Definition mod_semantic_judgement {A1 A2} c1 c2 w := *)
+(*     Spr1 (σ ⟨A1,A2⟩) ⟨c1,c2⟩ ≤ w. *)
 
-  Notation "⊨ c1 ≈ c2 [{ w }]" := (@mod_semantic_judgement _ _ c1 c2 w).
+(*   Notation "⊨ c1 ≈ c2 [{ w }]" := (@mod_semantic_judgement _ _ c1 c2 w). *)
 
-  Check (fun A B (c1 : M1 A) (c2: M2 B) w => ⊨ c1 ≈ c2 [{ w }] ).
+(*   Check (fun A B (c1 : M1 A) (c2: M2 B) w => ⊨ c1 ≈ c2 [{ w }] ). *)
 
-  Lemma weaken_rule {A B} {c1 : M1 A} {c2 : M2 B} {w w'} :
-    ⊨ c1 ≈ c2 [{ w }] -> w ≤ w' -> ⊨ c1 ≈ c2 [{ w' }].
-  Proof. move=> ? ? ; rewrite /mod_semantic_judgement ; estransitivity ; eassumption. Qed.
+(*   Lemma weaken_rule {A B} {c1 : M1 A} {c2 : M2 B} {w w'} : *)
+(*     ⊨ c1 ≈ c2 [{ w }] -> w ≤ w' -> ⊨ c1 ≈ c2 [{ w' }]. *)
+(*   Proof. move=> ? ? ; rewrite /mod_semantic_judgement ; estransitivity ; eassumption. Qed. *)
 
-  Lemma ret_rule {A B} {a : A} {b : B} :
-    ⊨ ret a ≈ ret b [{ Spr1 (η ⟨A,B⟩) ⟨a,b⟩ }].
-  Proof.
-    rewrite /mod_semantic_judgement.
-    move: (point_to_homomorphism_to_point Jprod rmW η ⟨A, B⟩ ⟨a,b⟩) => /= ->.
-    sreflexivity.
-  Qed.
+(*   Lemma ret_rule {A B} {a : A} {b : B} : *)
+(*     ⊨ ret a ≈ ret b [{ Spr1 (η ⟨A,B⟩) ⟨a,b⟩ }]. *)
+(*   Proof. *)
+(*     rewrite /mod_semantic_judgement. *)
+(*     move: (point_to_homomorphism_to_point Jprod rmW η ⟨A, B⟩ ⟨a,b⟩) => /= ->. *)
+(*     sreflexivity. *)
+(*   Qed. *)
 
-  Definition bindW {A1 A2 B1 B2}
-             (f1 : A1 -> M1 B1) (f2 : A2 -> M2 B2) (w : dfst (W ⟨A1,A2⟩)) :=
-    Spr1 (rm_bind rmW (to_prod f1 f2)) w.
+(*   Definition bindW {A1 A2 B1 B2} *)
+(*              (f1 : A1 -> M1 B1) (f2 : A2 -> M2 B2) (w : dfst (W ⟨A1,A2⟩)) := *)
+(*     Spr1 (rm_bind rmW (to_prod f1 f2)) w. *)
 
-  Lemma bind_act_rule {A1 A2 B1 B2}
-        {m1 : M1 A1} {m2 : M2 A2} {w} :
-    ⊨ m1 ≈ m2 [{ w }] -> forall (f1 : A1 -> M1 B1) (f2 : A2 -> M2 B2),
-      ⊨ bind m1 f1 ≈ bind m2 f2 [{ bindW f1 f2 w }].
-  Proof.
-    rewrite /mod_semantic_judgement.
-    move=> H f1 f2.
-    pose (rm_homo _ rmW σ (to_prod f1 f2) ⟨m1, m2⟩) as t.
-    move: t => /= ->. unfold bindW.
-    apply (Spr2 (rm_bind rmW (to_prod f1 f2)))=> //=.
-  Qed.
+(*   Lemma bind_act_rule {A1 A2 B1 B2} *)
+(*         {m1 : M1 A1} {m2 : M2 A2} {w} : *)
+(*     ⊨ m1 ≈ m2 [{ w }] -> forall (f1 : A1 -> M1 B1) (f2 : A2 -> M2 B2), *)
+(*       ⊨ bind m1 f1 ≈ bind m2 f2 [{ bindW f1 f2 w }]. *)
+(*   Proof. *)
+(*     rewrite /mod_semantic_judgement. *)
+(*     move=> H f1 f2. *)
+(*     pose (rm_homo _ rmW σ (to_prod f1 f2) ⟨m1, m2⟩) as t. *)
+(*     move: t => /= ->. unfold bindW. *)
+(*     apply (Spr2 (rm_bind rmW (to_prod f1 f2)))=> //=. *)
+(*   Qed. *)
 
-  Lemma if_rule {A1 A2} {m1: M1 A1} {m2 : M2 A2} {w w'} (b:bool) :
-      (if b then ⊨ m1 ≈ m2 [{ w }] else ⊨ m1 ≈ m2 [{ w' }])
-      -> ⊨ m1 ≈ m2 [{ if b then w else w' }].
-  Proof. destruct b=> //. Qed.
+(*   Lemma if_rule {A1 A2} {m1: M1 A1} {m2 : M2 A2} {w w'} (b:bool) : *)
+(*       (if b then ⊨ m1 ≈ m2 [{ w }] else ⊨ m1 ≈ m2 [{ w' }]) *)
+(*       -> ⊨ m1 ≈ m2 [{ if b then w else w' }]. *)
+(*   Proof. destruct b=> //. Qed. *)
 
-  Lemma nat_rect_rule {A1 A2} {m1: nat -> M1 A1} {m2 : nat -> M2 A2} {w0 wsuc}
-        (w := nat_rect (fun=> dfst (W ⟨A1, A2⟩)) w0 wsuc) :
-    ⊨ m1 0 ≈ m2 0 [{ w0 }] ->
-    (forall n, ⊨ m1 n ≈ m2 n [{ w n }] -> ⊨ m1 (S n) ≈ m2 (S n) [{ wsuc n (w n) }]) ->
-    forall n, ⊨ m1 n ≈ m2 n [{ w n }].
-  Proof. induction n => //=. apply H0=> //. Qed.
-    
-End RelationalProgramLogicFromBimodule.
+(*   Lemma nat_rect_rule {A1 A2} {m1: nat -> M1 A1} {m2 : nat -> M2 A2} {w0 wsuc} *)
+(*         (w := nat_rect (fun=> dfst (W ⟨A1, A2⟩)) w0 wsuc) : *)
+(*     ⊨ m1 0 ≈ m2 0 [{ w0 }] -> *)
+(*     (forall n, ⊨ m1 n ≈ m2 n [{ w n }] -> ⊨ m1 (S n) ≈ m2 (S n) [{ wsuc n (w n) }]) -> *)
+(*     forall n, ⊨ m1 n ≈ m2 n [{ w n }]. *)
+(*   Proof. induction n => //=. apply H0=> //. Qed. *)
+
+(* End RelationalProgramLogicFromBimodule. *)
 
 (* Generic rules for the simple framework [Section 2.4]*)
 
+Notation "wm ≫= wf" := (Spr1 (ord_relmon_bind _ wf) wm) (at level 50).
+
 Section RelationalProgramLogicFromRelativeMonadZero.
   Context (M1 M2 : Monad) (M12 := compPair M1 M2).
-  Context (W : RelationalSpecMonad0) `{BindMonotonicRelationalSpecMonad0 W}
+  Context (W : RelationalSpecMonad0)
           (θ : RelationalEffectObservation0 M1 M2 W).
-  
+
   Definition semantic_judgement A1 A2 c1 c2 w := Spr1 (θ ⟨A1,A2⟩) ⟨c1,c2⟩ ≤ w.
   Notation "⊨ c1 ≈ c2 [{ w }]" := (semantic_judgement _ _ c1 c2 w).
 
   Check (fun A B (c1 : M1 A) (c2: M2 B) w => ⊨ c1 ≈ c2 [{ w }] ).
+
 
   Import SPropNotations.
   Lemma seq_rule {A1 A2 B1 B2}
         {m1 : M1 A1} {m2 : M2 A2} {wm}
         {f1 : A1 -> M1 B1} {f2 : A2 -> M2 B2}
         {wf : OrdCat⦅Jprod ⟨A1,A2⟩ ; W ⟨B1, B2⟩⦆} :
-    ⊨ m1 ≈ m2 [{ wm }] -> (forall a1 a2, ⊨ f1 a1 ≈ f2 a2 [{ Spr1 wf ⟨a1, a2⟩ }]) ->
-    ⊨ bind m1 f1 ≈ bind m2 f2 [{ Spr1 (relmon_bind W wf) wm }].
+    ⊨ m1 ≈ m2 [{ wm }] -> (forall a1 a2, ⊨ f1 a1 ≈ f2 a2 [{ wf∙1 ⟨a1, a2⟩ }]) ->
+    ⊨ bind m1 f1 ≈ bind m2 f2 [{ wm ≫= wf }].
   Proof.
     intros Hm Hf.
-    rewrite /semantic_judgement.
-    move: (rmm_law2 _ _ M12 W θ _ _ (to_prod f1 f2) ⟨m1, m2⟩) => /= ->.
-    estransitivity.
-    apply (rsm0_bind_monotonic (θ ⟨B1, B2⟩ ∙ fmap Jprod (to_prod f1 f2)) wf) ; move=> [? ?] ; apply Hf.
-    eapply (Spr2 (relmon_bind W _) _ _)=> //.
+    rewrite /semantic_judgement; estransitivity.
+    apply: (rlmm_law2 _ _ M12 W θ _ _ (to_prod f1 f2) ⟨m1, m2⟩).
+    set f12 := ((θ _ ∙ _) ∙ _); estransitivity.
+    2: apply: (ord_relmon_bind_proper W _ _ f12); move=> [? ?] ; apply Hf.
+    apply: ((ord_relmon_bind W f12)∙2 _ _); apply: Hm.
   Qed.
-  
+
   Lemma weaken_rule2 {A B} {c1 : M1 A} {c2 : M2 B} {w w'} :
     ⊨ c1 ≈ c2 [{ w }] -> w ≤ w' -> ⊨ c1 ≈ c2 [{ w' }].
-  Proof. rewrite /semantic_judgement. move=> ? ? ; estransitivity ; eassumption.
+  Proof.
+    rewrite /semantic_judgement. move=> ? ? ; estransitivity ; eassumption.
   Qed.
 
   Lemma ret_rule2 {A B} {a : A} {b : B} :
-    ⊨ ret a ≈ ret b [{ Spr1 (relmon_unit W ⟨A , B⟩) ⟨a,b⟩ }].
+    ⊨ ret a ≈ ret b [{ (ord_relmon_unit W ⟨A , B⟩)∙1 ⟨a,b⟩ }].
   Proof.
-    rewrite /semantic_judgement.
-    cbv.
-    rewrite <- (rmm_law1 _ _ M12 W θ ⟨A , B⟩).
-    sreflexivity.
+    apply: (rlmm_law1 _ _ M12 W θ ⟨A , B⟩ ⟨a,b⟩).
   Qed.
 
 End RelationalProgramLogicFromRelativeMonadZero.
 
-  Notation "θ ⊨ c1 ≈ c2 [{ w }]" := (semantic_judgement _ _ _ θ _ _ c1 c2 w) (at level 85).
+Notation "θ ⊨ c1 ≈ c2 [{ w }]" := (semantic_judgement _ _ _ θ _ _ c1 c2 w) (at level 85).
 
 (* Tailored rules derived from the generic ones *)
 
 Section GoingPractical.
   Context (M1 M2 : Monad) (M12 := compPair M1 M2).
-  Context (W : RelationalSpecMonad0) `{BindMonotonicRelationalSpecMonad0 W}
-          (θ : RelationalEffectObservation0 M1 M2 W).
-  
+  Context (W : RelationalSpecMonad0) (θ : RelationalEffectObservation0 M1 M2 W).
+
   Lemma gp_ret_rule {A B a b w} :
-    Spr1 (relmon_unit W ⟨A , B⟩) ⟨a,b⟩ ≤ w ->
+    Spr1 (ord_relmon_unit W ⟨A , B⟩) ⟨a,b⟩ ≤ w ->
     θ ⊨ ret a ≈ ret b [{ w }].
   Proof. apply weaken_rule2 ; apply ret_rule2. Qed.
 
-  Lemma gp_seq_rule 
+  Lemma gp_seq_rule
         {A1 A2 B1 B2}
         {m1 : M1 A1} {m2 : M2 A2} {wm}
         {f1 : A1 -> M1 B1} {f2 : A2 -> M2 B2}
         {wf : OrdCat⦅Jprod ⟨A1,A2⟩ ; W ⟨B1, B2⟩⦆} {w} :
     θ ⊨ m1 ≈ m2 [{ wm }] ->
     (forall a1 a2, θ ⊨ f1 a1 ≈ f2 a2 [{ Spr1 wf ⟨a1, a2⟩ }]) ->
-    Spr1 (relmon_bind W wf) wm ≤ w ->
+    wm ≫= wf ≤ w ->
     θ ⊨ bind m1 f1 ≈ bind m2 f2 [{ w }].
   Proof. move=> ? ? ; apply weaken_rule2 ; apply seq_rule=> //. Qed.
 
@@ -143,31 +144,31 @@ Section GoingPractical.
 
   Definition skip {M:Monad} : M unit := ret tt.
   Notation "m1 ;; m2" := (bind m1 (fun=> m2)) (at level 65).
-  
+
   Lemma apply_left {A B1 B2} {m1 : M1 A} {c1 : M1 B1} {c2 : M2 B2} {w1 w2 w} :
     θ ⊨ m1 ≈ skip [{ w1 }] ->
     θ ⊨ c1 ≈ c2 [{ w2 }] ->
-    Spr1 (relmon_bind W (OrdCat_cst w2)) w1 ≤ w ->
+    w1 ≫= OrdCat_cst w2 ≤ w ->
     θ ⊨ m1 ;; c1 ≈ c2 [{ w }].
   Proof.
     move=> H1 H2 ; apply weaken_rule2.
     enough (c2 = skip ;; c2) as ->.
-    apply seq_rule=> //. 
+    apply seq_rule=> //.
     rewrite /bind monad_law1 //.
   Qed.
 
   Program Definition OrdCat_lift {A B} (f : A -> dfst B) : OrdCat⦅discr A; B⦆ :=
     Sexists _ f _.
   Next Obligation. move=> ? ? H0 ; induction H0; sreflexivity. Qed.
-  
+
   Program Definition OrdCat_lift' {A1 A2 B} (f : A1 -> A2 -> dfst B) : OrdCat⦅Jprod ⟨A1, A2⟩; B⦆ :=
     Sexists _ (fun a => f (nfst a) (nsnd a)) _.
   Next Obligation. move=> ? ? H0 ; induction H0; sreflexivity. Qed.
-  
+
   Lemma apply_left_tot {A1 A2} {c1 : M1 A1} {c2 : M2 A2} {w1 w2 w} :
     θ ⊨ c1 ≈ skip [{ w1 }] ->
     (forall a1, θ ⊨ ret a1 ≈ c2 [{ w2 a1 }]) ->
-    Spr1 (relmon_bind W (OrdCat_lift' (fun a=>fun=> w2 a))) w1 ≤ w ->
+    w1 ≫= OrdCat_lift' (fun a _ => w2 a) ≤ w ->
     θ ⊨ c1 ≈ c2 [{ w }].
   Proof.
     move=> H1 H2 ; apply weaken_rule2.
@@ -181,81 +182,81 @@ Section GoingPractical.
   Lemma apply_right {A B1 B2} {m2 : M2 A} {c1 : M1 B1} {c2 : M2 B2} {w1 w2 w} :
     θ ⊨ skip ≈ m2 [{ w1 }] ->
     θ ⊨ c1 ≈ c2 [{ w2 }] ->
-    Spr1 (relmon_bind W (OrdCat_cst w2)) w1 ≤ w ->
+    w1 ≫= OrdCat_cst w2 ≤ w ->
     θ ⊨ c1 ≈ m2 ;; c2 [{ w }].
   Proof.
     move=> H1 H2 ; apply weaken_rule2.
     enough (c1 = skip ;; c1) as ->.
-    apply seq_rule=> //. 
+    apply seq_rule=> //.
     rewrite /bind monad_law1 //.
   Qed.
 
   Lemma apply_right_tot {A1 A2} {c1 : M1 A1} {c2 : M2 A2} {w1 w2 w} :
     θ ⊨ skip ≈ c2 [{ w1 }] ->
     (forall a2, θ ⊨ c1 ≈ ret a2 [{ w2 a2 }]) ->
-    Spr1 (relmon_bind W (OrdCat_lift' (fun=>w2))) w1 ≤ w ->
+    w1 ≫= OrdCat_lift' (fun=>w2) ≤ w ->
     θ ⊨ c1 ≈ c2 [{ w }].
   Proof.
     move=> H1 H2 ; apply weaken_rule2.
     enough (c1 = skip ;; c1) as ->.
     enough (c2 = bind c2 ret) as ->.
-    apply seq_rule=> // ? ?; eapply weaken_rule2. 
+    apply seq_rule=> // ? ?; eapply weaken_rule2.
     rewrite /bind monad_law2 //.
     rewrite /bind monad_law1 //.
   Qed.
 
-  Let Wmod := rmon_morph_right_module W θ.
-  Let mod_semantic_judgement' {A1 A2} := 
-    @mod_semantic_judgement M1 M2 _ Wmod (rmon_unit W) A1 A2.
+  (* Let Wmod := rmon_morph_right_module W θ. *)
+  (* Let mod_semantic_judgement' {A1 A2} := *)
+  (*   @mod_semantic_judgement M1 M2 _ Wmod (rmon_unit W) A1 A2. *)
 
-  Import SPropNotations.
-  Lemma to_mod_semantic_judgement {A1 A2} {c1:M1 A1} {c2:M2 A2} w :
-    θ ⊨ c1 ≈ c2 [{ w }] -> mod_semantic_judgement' c1 c2 w.
-  Proof.
-    rewrite /mod_semantic_judgement'; unfold mod_semantic_judgement. 
-    unfold semantic_judgement.
-    enough (θ ⟨ A1, A2 ⟩ ∼ point_to_homomorphism Jprod Wmod (rmon_unit W) ⟨ A1, A2 ⟩) as -> => //.
-    cbv=> ? ; epose (relmon_law2 W) as t ; cbv in t ; rewrite t=> //.
-  Qed.
+  (* Import SPropNotations. *)
+  (* Lemma to_mod_semantic_judgement {A1 A2} {c1:M1 A1} {c2:M2 A2} w : *)
+  (*   θ ⊨ c1 ≈ c2 [{ w }] -> mod_semantic_judgement' c1 c2 w. *)
+  (* Proof. *)
+  (*   rewrite /mod_semantic_judgement'; unfold mod_semantic_judgement. *)
+  (*   unfold semantic_judgement. *)
+  (*   enough (θ ⟨ A1, A2 ⟩ ∼ point_to_homomorphism Jprod Wmod (rmon_unit W) ⟨ A1, A2 ⟩) as -> => //. *)
+  (*   cbv=> ? ; epose (relmon_law2 W) as t ; cbv in t ; rewrite t=> //. *)
+  (* Qed. *)
 
-  Lemma from_mod_semantic_judgement {A1 A2} {c1:M1 A1} {c2:M2 A2} w :
-    mod_semantic_judgement' c1 c2 w -> θ ⊨ c1 ≈ c2 [{ w }].
-  Proof.
-    rewrite /mod_semantic_judgement'; unfold mod_semantic_judgement. 
-    unfold semantic_judgement.
-    enough (θ ⟨ A1, A2 ⟩ ∼ point_to_homomorphism Jprod Wmod (rmon_unit W) ⟨ A1, A2 ⟩) as -> => //.
-    cbv=> ? ; epose (relmon_law2 W) as t ; cbv in t ; rewrite t=> //.
-  Qed.
+  (* Lemma from_mod_semantic_judgement {A1 A2} {c1:M1 A1} {c2:M2 A2} w : *)
+  (*   mod_semantic_judgement' c1 c2 w -> θ ⊨ c1 ≈ c2 [{ w }]. *)
+  (* Proof. *)
+  (*   rewrite /mod_semantic_judgement'; unfold mod_semantic_judgement. *)
+  (*   unfold semantic_judgement. *)
+  (*   enough (θ ⟨ A1, A2 ⟩ ∼ point_to_homomorphism Jprod Wmod (rmon_unit W) ⟨ A1, A2 ⟩) as -> => //. *)
+  (*   cbv=> ? ; epose (relmon_law2 W) as t ; cbv in t ; rewrite t=> //. *)
+  (* Qed. *)
 
-  Let act {A1 A2 B1 B2} := @bindW _ _ _ Wmod A1 A2 B1 B2.
-  Lemma cont_to_spec {A1 A2 B1 B2}
-        {m1 : M1 A1} {m2 : M2 A2} {w w'} :
-    θ ⊨ m1 ≈ m2 [{ w }] -> forall (f1 : A1 -> M1 B1) (f2 : A2 -> M2 B2),
-      act f1 f2 w ≤ w' ->
-      θ ⊨ bind m1 f1 ≈ bind m2 f2 [{ w' }].
-  Proof.
-    move=> ? ? ?; apply weaken_rule2 ; rewrite /act.
-    apply from_mod_semantic_judgement.
-    apply bind_act_rule; apply to_mod_semantic_judgement=> //.
-  Qed.
+  (* Let act {A1 A2 B1 B2} := @bindW _ _ _ Wmod A1 A2 B1 B2. *)
+  (* Lemma cont_to_spec {A1 A2 B1 B2} *)
+  (*       {m1 : M1 A1} {m2 : M2 A2} {w w'} : *)
+  (*   θ ⊨ m1 ≈ m2 [{ w }] -> forall (f1 : A1 -> M1 B1) (f2 : A2 -> M2 B2), *)
+  (*     act f1 f2 w ≤ w' -> *)
+  (*     θ ⊨ bind m1 f1 ≈ bind m2 f2 [{ w' }]. *)
+  (* Proof. *)
+  (*   move=> ? ? ?; apply weaken_rule2 ; rewrite /act. *)
+  (*   apply from_mod_semantic_judgement. *)
+  (*   apply bind_act_rule; apply to_mod_semantic_judgement=> //. *)
+  (* Qed. *)
 
-  (* This rule "shows" completeness of the simple rules using already defined rules
-     (and not unfolding the judgement which would be trivial,
-     a safer approach would consist in defining an inductive for ⊢)
-     assuming the bimodules rules, so not achieving much *)
-  Lemma to_spec {A1 A2} {m1 : M1 A1} {m2 : M2 A2} {w} :
-    Spr1 (θ ⟨_,_⟩) ⟨m1, m2⟩ ≤ w -> θ ⊨ m1 ≈ m2 [{ w }].
-  Proof.
-    enough (m1 = skip ;; m1) as ->.
-    enough (m2 = skip ;; m2) as ->.
-    enough (Spr1 (θ ⟨_,_⟩) ⟨skip ;; m1, skip ;; m2⟩ = act (fun=> m1) (fun=> m2) (Spr1 (rmon_unit W ⟨_,_⟩) ⟨tt,tt⟩)) as ->.
-    apply cont_to_spec.
-    rewrite /skip ; apply ret_rule2.
-    move: (rmm_law2 _ _ _ _ θ _ _ (to_prod (fun=> m1) (fun=> m2)) ⟨skip,skip⟩)
-    => /= ->.
-    move: (rmm_law1 _ _ _ _ θ ⟨_,_⟩ ⟨tt,tt⟩) => /= -> //.
-    all:rewrite /bind monad_law1 //.
-  Qed.
+  (* (* This rule "shows" completeness of the simple rules using already defined rules *)
+  (*    (and not unfolding the judgement which would be trivial, *)
+  (*    a safer approach would consist in defining an inductive for ⊢) *)
+  (*    assuming the bimodules rules, so not achieving much *) *)
+  (* Lemma to_spec {A1 A2} {m1 : M1 A1} {m2 : M2 A2} {w} : *)
+  (*   Spr1 (θ ⟨_,_⟩) ⟨m1, m2⟩ ≤ w -> θ ⊨ m1 ≈ m2 [{ w }]. *)
+  (* Proof. *)
+  (*   enough (m1 = skip ;; m1) as ->. *)
+  (*   enough (m2 = skip ;; m2) as ->. *)
+  (*   enough (Spr1 (θ ⟨_,_⟩) ⟨skip ;; m1, skip ;; m2⟩ = act (fun=> m1) (fun=> m2) (Spr1 (rmon_unit W ⟨_,_⟩) ⟨tt,tt⟩)) as ->. *)
+  (*   apply cont_to_spec. *)
+  (*   rewrite /skip ; apply ret_rule2. *)
+  (*   move: (rmm_law2 _ _ _ _ θ _ _ (to_prod (fun=> m1) (fun=> m2)) ⟨skip,skip⟩) *)
+  (*   => /= ->. *)
+  (*   move: (rmm_law1 _ _ _ _ θ ⟨_,_⟩ ⟨tt,tt⟩) => /= -> //. *)
+  (*   all:rewrite /bind monad_law1 //. *)
+  (* Qed. *)
 
 End GoingPractical.
 
